Finishing merge TransitionSystems.v

theories/Labelled_Transition_System/Examples_of_LTS/VACCS/VACCS_Examples.v
@@ -31,17 +31,17 @@ From Must Require Import InputOutputActions ActTau OldTransitionSystems Must VAC
 gLts Bisimulation Lts_OBA Lts_FW Lts_OBA_FB GeneralizeLtsOutputs ParallelLTSConstruction ForwarderConstruction
 InteractionBetweenLts Testing_Predicate.
 (************************************* Examples for VACCS *************************************)
-Parameter c : Channel.
+Parameter a : Channel.
 Parameter O : Value.
 Parameter I : Value.
 Parameter (neq : O ≠ I).
 
-Definition p : proc := c ? x • (c ! O • 𝟘).
+Definition cst : proc := a ? x • (a ! O • 𝟘).
 
-Definition q : proc := c ? x • (c ! (bvar 0) • 𝟘).
+Definition ccat : proc := a ? x • (a ! (bvar 0) • 𝟘).
 
-Lemma q_is_above_NIL : 
-  (@ctx_pre _ _ _ _ _ _ proc _ _ _ _ _ _ _ (g 𝟘) q). (* 𝟘 ⊑ₘᵤₛₜᵢ q *)
+Lemma copycat_is_above_NIL : 
+  (@ctx_pre _ _ _ _ _ _ proc _ _ _ _ _ _ _ (g 𝟘) ccat). (* 𝟘 ⊑ₘᵤₛₜᵢ ccat *)
 Proof.
   intros e Hyp.
   dependent induction Hyp.
@@ -49,7 +49,7 @@ Proof.
   - eapply m_step; eauto.
     + inversion ex; subst. inversion H2; subst.
       * inversion l.
-      * exists (q ▷ b2). eapply ParRight. eauto.
+      * exists (ccat ▷ b2). eapply ParRight. eauto.
       * inversion l1.
     + intros. eauto. inversion H2.
     + intros. destruct μ1 as [ (*Input*) a | (*Output*) a ].
@@ -61,12 +61,12 @@ Proof.
            ++ inversion ex. inversion H2; subst.
               ** inversion l.
               ** unfold lts_step in l; simpl in *.
-                 assert (lts e ((c ⋉ v) !) e') as HypTr; eauto.
+                 assert (lts e ((a ⋉ v) !) e') as HypTr; eauto.
                  eapply OBA_with_FB_Fifth_Axiom in HypTr 
                     as [(e'' & HypTr' & e'0 & HypTr'0 & equiv')|(e'' & HypTr' & equiv'')]; eauto.
-                 --- exists (c ! v • 𝟘 ▷ e''). eapply ParRight. eauto.
-                 --- assert (lts (c ! v • 𝟘) ((c ⋉ v) !) (g 𝟘)).
-                     { eauto with ccs. }
+                 --- exists (a ! v • 𝟘 ▷ e''). eapply ParRight. eauto.
+                 --- assert (lts (a ! v • 𝟘) ((a ⋉ v) !) (g 𝟘)).
+                     { eauto with cgr. }
                       exists ((g 𝟘) ▷ e''). eapply ParSync; eauto.
                      simpl; eauto.
               ** inversion l1.
@@ -80,8 +80,8 @@ Proof.
                  { eapply unoutcome_preserved_by_eq; eauto. }
                  assert (¬ good_VACCS e1) as not_happy''.
                  { eapply unoutcome_preserved_by_lts_non_blocking_action_converse; eauto.
-                   unfold non_blocking; simpl. exists (c ⋉ v); eauto. }
-                 assert (must q e1); eauto.
+                   unfold non_blocking; simpl. exists (a ⋉ v); eauto. }
+                 assert (must ccat e1); eauto.
                  eapply must_preserved_by_synch_if_notoutcome; eauto.
                  simpl; eauto.
            ++ intros. inversion H5; subst. simpl in *.
@@ -91,11 +91,11 @@ Proof.
       * inversion H3.
 Qed.
 
-Lemma NIL_is_above_q : 
-  (@ctx_pre _ _ _ _ _ _ proc _ _ _ _ _ _ _ q (g 𝟘)). (* q ⊑ₘᵤₛₜᵢ 𝟘 *)
+Lemma NIL_is_above_copycat : 
+  (@ctx_pre _ _ _ _ _ _ proc _ _ _ _ _ _ _ ccat (g 𝟘)). (* ccat ⊑ₘᵤₛₜᵢ 𝟘 *)
 Proof.
   intros e Hyp.
-  assert (must q e) as Mq; eauto.
+  assert (must ccat e) as Mq; eauto.
   dependent induction Hyp.
   - now eapply m_now.
   - inversion ex. inversion H2; subst.
@@ -108,7 +108,7 @@ Proof.
       * intros. inversion H4.
     + inversion l1; subst.
       eapply simplify_match_input in eq. subst.
-      assert (must ((c ! (bvar 0) • 𝟘) ^ v) b2) as Mq'.
+      assert (must ((a ! (bvar 0) • 𝟘) ^ v) b2) as Mq'.
       { eapply must_preserved_by_synch_if_notoutcome ; eauto. simpl; eauto. }
       inversion Mq'.
       * assert (good_VACCS e).
@@ -132,8 +132,8 @@ Proof.
            ++ intros. inversion H5.
 Qed.
 
-Lemma q_is_above_p : 
-  (@ctx_pre _ _ _ _ _ _ proc _ _ _ _ _ _ _ p q). (* p ⊑ₘᵤₛₜᵢ q *)
+Lemma copycat_is_above_constant : 
+  (@ctx_pre _ _ _ _ _ _ proc _ _ _ _ _ _ _ cst ccat). (* cst ⊑ₘᵤₛₜᵢ ccat *)
 Proof.
   intros e HypMust.
   dependent induction HypMust.
@@ -141,31 +141,31 @@ Proof.
   - eapply m_step; eauto.
     + inversion ex; subst. inversion H2; subst.
       * inversion l.
-      * exists (q ▷ b2). eapply ParRight. eauto.
+      * exists (ccat ▷ b2). eapply ParRight. eauto.
       * inversion l1; subst.
         eapply simplify_match_input in eq as eq'; subst.
         eexists. eapply ParSync; eauto.
-        unfold q. eapply lts_input; eauto.
+        unfold ccat. eapply lts_input; eauto.
     + intros. eauto. inversion H2.
     + intros. inversion H3; subst.
       eapply simplify_match_input in H2 as eq;subst.
       assert (¬ good_VACCS e') as not_happy'.
       { eapply unoutcome_preserved_by_lts_non_blocking_action; eauto.
-        exists (c ⋉ v); eauto. }
+        exists (a ⋉ v); eauto. }
       eapply m_step; eauto.
-      * assert (must ((c ! O • 𝟘) ^ v) e') as Mp'.
-        { eapply (must_preserved_by_synch_if_notoutcome p _ e _) ; eauto.
+      * assert (must ((a ! O • 𝟘) ^ v) e') as Mp'.
+        { eapply (must_preserved_by_synch_if_notoutcome cst _ e _) ; eauto.
           eapply m_step; eauto. eapply lts_input. }
         inversion Mp'. contradiction.
         inversion ex0. inversion H5; subst.
         -- inversion l.
-        -- exists ((c ! 0 • 𝟘) ^ v ▷ b2). eapply ParRight; eauto.
+        -- exists ((a ! 0 • 𝟘) ^ v ▷ b2). eapply ParRight; eauto.
         -- inversion l1; subst. eapply simplify_match_output in eq as eq'; subst.
-           assert (e' ⟶[ActIn (c ⋉ O)] b2) as l'2; eauto.
+           assert (e' ⟶[ActIn (a ⋉ O)] b2) as l'2; eauto.
            eapply TransitionShapeForInput in l2 as (p1 & g1 & r1 & n & equiv1 & equiv2 & eq1).
            edestruct (Congruence_Respects_Transition e') as (e'1 & Tr'1 & equiv'1). 
-           { exists (Ѵ n (((gpr_input c p1 + g1) ‖ r1))). split; eauto. eapply lts_res_ext_n. eapply lts_parL.
-             eapply lts_choiceL. instantiate (2 := ActIn (c ⋉ v)). simpl. eapply lts_input. }
+           { exists (Ѵ n (((gpr_input a p1 + g1) ‖ r1))). split; eauto. eapply lts_res_ext_n. eapply lts_parL.
+             eapply lts_choiceL. instantiate (2 := ActIn (a ⋉ v)). simpl. eapply lts_input. }
            simpl. exists (g 𝟘 , e'1). eapply ParSync.
            ++ symmetry in H2. exact H2.
            ++ eapply lts_output.
@@ -179,26 +179,26 @@ Proof.
            { eapply unoutcome_preserved_by_eq; eauto. }
            assert (¬ good_VACCS e1) as not_happy'''.
            { eapply unoutcome_preserved_by_lts_non_blocking_action_converse; eauto.
-             unfold non_blocking; simpl. exists (c ⋉ v); eauto. }
-           assert (must q e1); eauto.
+             unfold non_blocking; simpl. exists (a ⋉ v); eauto. }
+           assert (must ccat e1); eauto.
            eapply must_preserved_by_synch_if_notoutcome; eauto.
       * intros. inversion H6; subst.
         eapply simplify_match_output in H5 as eq; subst.
-        assert (lts e ((c ⋉ v) !) e') as l2; eauto.
+        assert (lts e ((a ⋉ v) !) e') as l2; eauto.
         eapply OBA_with_FB_Fourth_Axiom in l2 as (e'1 & HypTr'1 & equiv1); eauto.
-        eapply must_eq_client; eauto. assert (must p e) as Mp. eapply m_step; eauto.
-        assert (must p e'1) as Mp';eauto.
-        assert (must q e'1); eauto. eapply NIL_is_above_q. eauto.
+        eapply must_eq_client; eauto. assert (must cst e) as Mp. eapply m_step; eauto.
+        assert (must cst e'1) as Mp';eauto.
+        assert (must ccat e'1); eauto. eapply NIL_is_above_copycat. eauto.
 Qed.
 
 
 Lemma NIL_is_above_p : 
-  (@ctx_pre _ _ _ _ _ _ proc _ _ _ _ _ _ _ p (g 𝟘)). (* p ⊑ₘᵤₛₜᵢ 𝟘 *)
+  (@ctx_pre _ _ _ _ _ _ proc _ _ _ _ _ _ _ cst (g 𝟘)). (* cst ⊑ₘᵤₛₜᵢ 𝟘 *)
 Proof.
-  intros e Hyp. eapply NIL_is_above_q. eapply q_is_above_p. exact Hyp.
+  intros e Hyp. eapply NIL_is_above_copycat. eapply copycat_is_above_constant. exact Hyp.
 Qed.
 
-Definition Test := (c ! I • 𝟘) ‖ (c ? x • (If (bvar 0 == I) Then ① Else (g 𝟘))).
+Definition Test := (a ! I • 𝟘) ‖ (a ? x • (If (bvar 0 == I) Then ① Else (g 𝟘))).
 
 Lemma this_Test_is_not_good : ¬ good_VACCS Test.
 Proof.
@@ -212,7 +212,7 @@ Proof.
   eapply m_step.
   - eapply this_Test_is_not_good.
   - exists (g 𝟘 ▷ (g 𝟘 ‖ ((If (bvar 0 == I) Then ① Else (g 𝟘))^I))).
-    eapply ParRight. eapply lts_comL; eauto with ccs.
+    eapply ParRight. eapply lts_comL; eauto with cgr.
   - intros ? imp. inversion imp.
   - intros. inversion H; subst.
     + inversion H3; subst. simpl. inversion H2; subst.
@@ -225,15 +225,15 @@ Proof.
 Qed.
 
 
-Lemma p_is_not_above_NIL : 
-¬ (@ctx_pre _ _ _ _ _ _ proc _ _ _ _ _ _ _ (g 𝟘) p). (* ¬ 𝟘 ⊑ₘᵤₛₜᵢ p *)
+Lemma constant_is_not_above_NIL : 
+¬ (@ctx_pre _ _ _ _ _ _ proc _ _ _ _ _ _ _ (g 𝟘) cst). (* ¬ 𝟘 ⊑ₘᵤₛₜᵢ cst *)
 Proof.
   intro imp.
-  assert (must p Test).
+  assert (must cst Test).
   { eapply imp. eapply NIL_must_this_TEST. }
   inversion H.
   + eapply this_Test_is_not_good; eauto.
-  + assert (must ((c ! O • 𝟘)^I) ((g 𝟘) ‖ (c ? x • (If (bvar 0 == I) Then ① Else (g 𝟘))))) as Mp.
+  + assert (must ((a ! O • 𝟘)^I) ((g 𝟘) ‖ (a ? x • (If (bvar 0 == I) Then ① Else (g 𝟘))))) as Mp.
     { eapply com; eauto. 2: { eapply lts_input. } 2: { eapply lts_parL. eapply lts_output. }
     simpl; eauto. }
     simpl in Mp.
@@ -261,12 +261,12 @@ Proof.
 Qed.
 
 Lemma p_is_not_above_q : 
-  ¬ (@ctx_pre _ _ _ _ _ _ proc _ _ _ _ _ _ _ q p). (* ¬ q ⊑ₘᵤₛₜᵢ p *)
+  ¬ (@ctx_pre _ _ _ _ _ _ proc _ _ _ _ _ _ _ ccat cst). (* ¬ ccat ⊑ₘᵤₛₜᵢ cst *)
 Proof.
-  intros imp. assert (@ctx_pre _ _ _ _ _ _ proc _ _ _ _ _ _ _ (g 𝟘) q) as HypMust.
-  { eapply q_is_above_NIL; eauto. }
-  assert (@ctx_pre _ _ _ _ _ _ proc _ _ _ _ _ _ _ (g 𝟘) p) as imp'.
+  intros imp. assert (@ctx_pre _ _ _ _ _ _ proc _ _ _ _ _ _ _ (g 𝟘) ccat) as HypMust.
+  { eapply copycat_is_above_NIL; eauto. }
+  assert (@ctx_pre _ _ _ _ _ _ proc _ _ _ _ _ _ _ (g 𝟘) cst) as imp'.
   { intros e HM. eapply imp. eapply HypMust. eauto. }
-  assert (¬ (@ctx_pre _ _ _ _ _ _ proc _ _ _ _ _ _ _ (g 𝟘) p)). { eapply p_is_not_above_NIL. }
+  assert (¬ (@ctx_pre _ _ _ _ _ _ proc _ _ _ _ _ _ _ (g 𝟘) cst)). { eapply constant_is_not_above_NIL. }
   contradiction.
 Qed.
